fstar/test/MLS.Test.FromExt.PreSharedKeys.fst
@@ -1,0 +1,41 @@
+module MLS.Test.FromExt.PreSharedKeys
+
+open FStar.IO
+open FStar.All
+open Comparse
+open MLS.Test.Types
+open MLS.Test.Utils
+open MLS.StringUtils
+
+open MLS.Result
+open MLS.Crypto
+open MLS.TreeDEM.PSK
+
+val test_psk_one: psk_test -> ML bool
+let test_psk_one t =
+  match uint16_to_ciphersuite t.cipher_suite with
+  | ProtocolError s -> begin
+    IO.print_string ("Skipping one test because of missing ciphersuite: '" ^ s ^ "'\n");
+    true
+  end
+  | InternalError s -> begin
+    IO.print_string ("Internal error! '" ^ s ^ "'\n");
+    false
+  end
+  | Success cs -> begin
+    let cb = mk_concrete_crypto_bytes cs in
+    let psk_data =
+      List.map
+        (fun psk -> ({
+          id = PSKI_external (hex_string_to_bytes psk.psk_id);
+          nonce = (hex_string_to_bytes psk.psk_nonce);
+        }, hex_string_to_bytes psk.psk))
+        t.psks
+    in
+    let psk_secret = extract_result (compute_psk_secret psk_data) in
+    check_equal "psk_secret" (bytes_to_hex_string) (hex_string_to_bytes t.psk_secret) (psk_secret)
+  end
+
+val test_psk: list psk_test -> ML bool
+let test_psk =
+  test_list "Pre-Shared Keys" test_psk_one
